{
 "cells": [
  {
   "cell_type": "markdown",
   "metadata": {},
   "source": [
    "### 2.1.2 Binomial Coefficients and the Binomial Theorem\n",
    "#### 73 Use the fact that $(x+y)^n = (x+y)(x+y)^{n-1}$ to give an inductive proof of the binomial theorem.\n",
    "The claim is that $(x+y)^n = \\sum_{i=0}^n \\binom{n}{i}x^i y^{n-i}$ for each nonnegative integer $n$. The base case is for $n=0$ and in this case the relation holds since\n",
    "$$(x+y)^0 = 1 = \\sum_{i=0}^0 \\binom{0}{i} x^i y^{0-i} 1.$$\n",
    "\n",
    "Now assume the relation holds for some integer $n-1$ and we prove that it holds for $n$:\n",
    "$$\\begin{align*}\n",
    "(x+y)^n = (x+y)(x+y)^{n-1} &= (x+y) \\sum_{i=0}^{n-1}\\binom{n-1}{i} x^i y^{n-1-i} \\\\\n",
    "&= \\sum_{i=0}^{n-1}\\binom{n-1}{i} x^{i+1} y^{n-1-i} + \\sum_{i=0}^{n-1}\\binom{n-1}{i} x^i y^{n-i} \\quad \\text{(distribute $x$ and $y$)}\\\\\n",
    "&= \\sum_{i=1}^{n} \\binom{n-1}{i-1}x^i y^{n-i} + \\sum_{i=0}^{n-1}\\binom{n-1}{i}x^i y^{n-i} \\quad \\text{(shift index of first sum)}\\\\\n",
    "&= \\sum_{i=1}^{n-1} \\left(\\binom{n-1}{i-1} + \\binom{n-1}{i}\\right)x^i y^{n-1} + \\binom{n-1}{n-1}x^ny^0 + \\binom{n-1}{0}x^0y^n \\quad \\text{(rewrite sums and factor)}\\\\\n",
    "&= \\sum_{i=1}^{n-1}\\binom{n}{i}x^i y^{n-i} + \\binom{n}{n}x^n y^{n-n} + \\binom{n}{0}x^0y^n \\quad \\text{(pascal identity and rewrite coefs of last two terms)}\\\\\n",
    "&= \\sum_{i=0}^n \\binom{n}{i}x^i y^{n-i} \\quad \\text{(combine into one sum)}\n",
    "\\end{align*}$$\n",
    "\n",
    "#### 74 Suppose that $f$ is a function defined on the nonnegative integers such that $f(0) = 3$ and $f(n) = 2f(n − 1)$. Find a formula for $f(n)$ and prove your formula is correct.\n",
    "Claim: $f(n) = 3\\cdot 2^n$ for $n=0,1,2\\cdots$. Proof is done by induction on $n$. The base case is $n=1$ which holds since\n",
    "$$f(1) = 3\\cdot 2 = 6 = 2\\cdot 3 \\cdot 2^0 = 2f(0).$$\n",
    "Now inductively assume that $f(n-1)=3\\cdot 2^{n-1}$ so that the hypothesis holds for some integer $n-1$. Then we have\n",
    "$$f(n) = 2 f(n-1) = 2\\cdot 3\\cdot 2^{n-1} = 3\\cdot 2^{n}$$\n",
    "\n",
    "### 2.2 Recurrence Relations\n",
    "#### 87 How is the number of subsets of an $n$-element set related to the number of subsets of an $(n − 1)$-element set?\n",
    "The number of $n$ element subsets is equal to the number of $(n-1)$-element subsets multiplied by $2$. The reasoning is that if we take a set $S$ with $(n-1)$-elements, from previous problems we know that there are $2^{n-1}$ subsets. Denote the set of subsets as $P_S$. If we then add one more element to $S$, say $x$, and we want to construct the new set of subsets $P_{S'}$, then we must either add or withold $x$ from each of the sets in $P_S$. In other words, $P_{S'}$ will contain all of the same elements of $P_S$, plus all of the sets from $P_S$ with $x$ added in. \n",
    "\n",
    "The recurrence relation is thus $S_n = 2 S_{n-1}$, where $S_0=1$. The claim is that $S_n = 2^{n}$ and the proof is done by induction on $n$. The base case is $n=1$ which holds since a set with $1$ elements has, $2^1$ subsets -- one set containing the element and the other being the empty set. Now inductively assume that $S_{n-1} = 2^{n-1}$ so that the relation holds for some integer $n-1$. Then we have\n",
    "$$S_n = 2 \\cdot S_{n-1} = 2 \\cdot 2^{n-1} = 2^n.$$\n",
    "\n",
    "#### 88  Explain why it is that the number of bijections from an $n$-element set to an $n$-element set is equal to $n$ times the number of bijections from an $(n − 1)$-element subset to an $(n − 1)$-element set.\n",
    "The number of bijections from an $(n-1)$ element set to an $(n-1)$ element set is equal to $(n-1)!$ which we have shown previously. The reasoning being that the number of bijections is equal to product of the sequence of $n-1$ assignments to be made on the $n-1$ elements, i.e. $n-1$ choices to map the first element to $n-2$ choices to map the second element to and so on and so forth.\n",
    "\n",
    "Thus the number of bijections from an $n$-element set to an $n$-element set is $n! = n \\cdot (n-1)!$. The recurrence relation is given by $B_n = n B_{n-1}$ with $B_0=1$ and the claim is that $B_n = n!$. The proof is done by induction on $n$. The base case holds for $n=1$ since \n",
    "$$B_1 = 1\\cdot B_0 = 1 = 1!.$$\n",
    "Now inductively assume that $B_{n-1}=(n-1)!$ for some integer $n-1$. Then we have \n",
    "$$B_n = n \\cdot B_{n-1} = n \\cdot (n-1)! = n!$$\n",
    "\n",
    "### 2.2.2 Arithmetic Series\n",
    "#### 93 A child puts away two dollars from her allowance each week. If she starts with twenty dollars, give a recurrence for the amount $a_n$ of money she has after $n$ weeks and find out how much money she has at the end of $n$ weeks.\n",
    "The recurrence is $a_n = 2 + a_{n-1}$ with $a_0 = 20$ since she start with $20$ dollars. The solution to the recurrence is $a_n = 20 + 2n$. Proof by induction: base case $n=1$ holds since\n",
    "$$a_1 = 2+a_0 = 2+20 = 22 = 20 + 2\\cdot1 = 22.$$\n",
    "Now inductively assume that $a_{n-1} = 20 + 2(n-1)$ for some integer $n-1$ and we have\n",
    "$$a_n = 2 + a_{n-1} = 2 + 20 + 2(n-1) = 20 + 2n - 2 + 2 = 20 + 2n$$\n",
    "\n",
    "#### 94 A sequence that satisfies a recurrence of the form $a_n = a_{n−1} + c$ is called an *arithmetic progression*. Find a formula in terms of the initial value $a_0$ and the common difference $c$ for the term an in an arithmetic progression and prove you are right.\n",
    "The claim is that $a_n = a_0 + cn$ and the proof is done by induction on $n$. The base case happens when $n=1$ and is true since \n",
    "$$a_1 = a_0 + c.$$\n",
    "Now inductively assume that $a_{n-1} = a_0 + c(n-1)$ for some integer $n-1$ and we have\n",
    "$$a_n = a_{n-1} + c = a_0 + c(n-1) + c = a_0 + cn - c + c = a_0 + cn.$$\n",
    "\n",
    "#### 95 A person who is earning \\$ $50,000$ per year gets a raise of \\$ $3000$ a year for $n$ years in a row. Find a recurrence for the amount $a_n$ of money the person earns over $n + 1$ years. What is the total amount of money that the person earns over a period of $n + 1$ years? (In $n+1$ years there are $n$ raises)\n",
    "From the previous exercise we know that the persons salary for the $n^{th}$ year is given by $a_n = 3000n + 50000$. Thus the total money earned in $n+1$ years is equal to the the sum of the salaries earned each year \n",
    "$$s_{n} = \\sum_{i=0}^n a_i = \\sum_{i=0}^n \\left(3000n + 50000\\right)$$\n",
    "\n",
    "#### 96 An *arithmetic series* is a sequence $s_n$ equal to the sum of the terms $a_0$ through $a_n$ of an arithmetic progression. Find a recurrence for the sum $s_n$ of an arithmetic progression with initial value $a_0$ and common difference $c$ (using the language of Problem 94). Find a formula for general term $s_n$ of an arithmetic series.\n",
    "The recursion is given by \n",
    "$$s_{n} = s_{n-1} + a_n = s_{n-1} + a_0 + nc, \\ s_0 = a_0,$$\n",
    "and the solution is given by \n",
    "$$s_n = \\frac{(n+1)(a_0 + a_{n})}{2}$$.\n",
    "\n",
    "The proof is done by induction on $n$ and the base case holds since \n",
    "$$\n",
    "\\begin{align*}\n",
    "s_1 &= 2\\frac{(a_0 + a_1)}{2} = a_0 + a_1 \\\\\n",
    "s_1 &= s_{0} + a_1 =a_0 + a_1.\n",
    "\\end{align*}$$\n",
    "Now inductively assume that $s_{n-1} = \\frac{n(a_0 + a_{n-1})}{2}$ for some integer $n-1$ and we have that\n",
    "$$\n",
    "\\begin{align*}\n",
    "s_n = s_{n-1} + a_n = \\frac{n(a_0 + a_{n-1})}{2} + a_n = \\frac{n(a_0 + a_0 + (n-1)c)+ 2a_n}{2}  &= \\frac{na_0 + na_n -nc+2a_0 + 2nc}{2} \\\\\n",
    "&= \\frac{na_0 + a_0 + na_n + a_n}{2} \\\\\n",
    "&= \\frac{(n+1)(a_0 + a_n)}{2}.\n",
    "\\end{align*}$$\n",
    "\n",
    "\n",
    "### 2.2.3 First Order Linear Recurrences\n",
    "#### 98 Find a formula in terms of $b$, $d$, $a_0$ and $n$ for the general term $a_n$ of a sequence that satisfies a constant coefficient first order linear recurrence $a_n = ba_{n−1} + d$ and prove you are correct.\n",
    "The claim is that \n",
    "$$a_n = b^n a_0 + \\sum_{i=0}^{n-1}d b^i = b^n a_0 + d\\frac{1-b^n}{1-b}$$ \n",
    "and the proof is done by induction on $n$. The base case holds since \n",
    "$$a_1 = b a_0 +d = b^1 a_0 + d\\frac{1-b^1}{1-b} = b^1 a_0 + d.$$\n",
    "Now inductively assume that $a_{n-1} = b^{n-1}a_0 + \\sum_{i=0}^{n-2}db^i$ for some integer $n-1$ and then we have that\n",
    "$$\\begin{align*}\n",
    "a_n = b a_{n-1} + d = b \\left(b^{n-1}a_0 + \\sum_{i=0}^{n-2}db^i\\right) + d =& b^na_0 + \\sum_{i=0}^{n-2}db^{i+1} + d \\\\\n",
    "&= b^na_0 + \\sum_{i=1}^{n-1}db^i + db^0 \\quad \\text{(shift indices)} \\\\\n",
    "&= b^n a_0 + \\sum_{i=0}^{n-1}d b^i \\quad \\text{(add third term into sum)}\\\\\n",
    "&= b^n a_0 + d\\frac{1-b^{n}}{1-b} \\quad \\text{(simplify sum of geometric series)}\n",
    "\\end{align*}$$"
   ]
  }
 ],
 "metadata": {
  "kernelspec": {
   "display_name": "Python 2",
   "language": "python",
   "name": "python2"
  },
  "language_info": {
   "codemirror_mode": {
    "name": "ipython",
    "version": 2
   },
   "file_extension": ".py",
   "mimetype": "text/x-python",
   "name": "python",
   "nbconvert_exporter": "python",
   "pygments_lexer": "ipython2",
   "version": "2.7.13"
  }
 },
 "nbformat": 4,
 "nbformat_minor": 2
}
